theories/lifetime/model/definitions.v
@@ -66,7 +66,7 @@ Definition lftGpreS' := lftGpreS.
 Definition lftΣ : gFunctors :=
   #[ boxΣ; GFunctor (authR alftUR); GFunctor (authR ilftUR);
      GFunctor (authR borUR); GFunctor (authR natUR); GFunctor (authR inhUR) ].
-Instance subG_lftGpreS Σ :
+Global Instance subG_lftGpreS Σ :
   subG lftΣ Σ → lftGpreS Σ.
 Proof. solve_inG. Qed.
 
@@ -200,12 +200,12 @@ Section defs.
     (∃ κ', lft_incl κ κ' ∗ raw_bor κ' P)%I.
 End defs.
 
-Instance: Params (@lft_bor_alive) 4 := {}.
-Instance: Params (@lft_inh) 5 := {}.
-Instance: Params (@lft_vs) 4 := {}.
-Instance idx_bor_params : Params (@idx_bor) 5 := {}.
-Instance raw_bor_params : Params (@raw_bor) 4 := {}.
-Instance bor_params : Params (@bor) 4 := {}.
+Global Instance: Params (@lft_bor_alive) 4 := {}.
+Global Instance: Params (@lft_inh) 5 := {}.
+Global Instance: Params (@lft_vs) 4 := {}.
+Global Instance idx_bor_params : Params (@idx_bor) 5 := {}.
+Global Instance raw_bor_params : Params (@raw_bor) 4 := {}.
+Global Instance bor_params : Params (@bor) 4 := {}.
 
 Notation "q .[ κ ]" := (lft_tok q κ)
     (format "q .[ κ ]", at level 2, left associativity) : bi_scope.
