theories/lifetime/model/primitive.v
@@ -254,14 +254,14 @@ Proof.
 Qed.
 
 (** Basic rules about lifetimes  *)
-Instance lft_inhabited : Inhabited lft := _.
-Instance bor_idx_inhabited : Inhabited bor_idx := _.
-Instance lft_intersect_comm : Comm (A:=lft) eq (⊓) := _.
-Instance lft_intersect_assoc : Assoc (A:=lft) eq (⊓) := _.
-Instance lft_intersect_inj_1 κ : Inj eq eq (κ ⊓.) := _.
-Instance lft_intersect_inj_2 κ : Inj eq eq (.⊓ κ) := _.
-Instance lft_intersect_left_id : LeftId eq static (⊓) := _.
-Instance lft_intersect_right_id : RightId eq static (⊓) := _.
+Local Instance lft_inhabited : Inhabited lft := _.
+Local Instance bor_idx_inhabited : Inhabited bor_idx := _.
+Local Instance lft_intersect_comm : Comm (A:=lft) eq (⊓) := _.
+Local Instance lft_intersect_assoc : Assoc (A:=lft) eq (⊓) := _.
+Local Instance lft_intersect_inj_1 κ : Inj eq eq (κ ⊓.) := _.
+Local Instance lft_intersect_inj_2 κ : Inj eq eq (.⊓ κ) := _.
+Local Instance lft_intersect_left_id : LeftId eq static (⊓) := _.
+Local Instance lft_intersect_right_id : RightId eq static (⊓) := _.
 
 Lemma lft_tok_sep q κ1 κ2 : q.[κ1] ∗ q.[κ2] ⊣⊢ q.[κ1 ⊓ κ2].
 Proof. by rewrite /lft_tok -big_sepMS_disj_union. Qed.
